clock_sorted

high/Veritas.Interleave.fst
@@ -851,8 +851,24 @@ let interleave_sseq_index (#a:eqtype) (il:interleaving a) (i:seq_index il)
     let tid, j = i2s_map il i in
     Seq.index (s_seq il_i) tid `Seq.equal`
     SA.prefix (Seq.index (s_seq il) tid) j)
-  = let il_i = prefix il i in
+  = i2s_prefix_length il i
+
+let rec interleave_sseq_index_next (#a:eqtype) (il:interleaving a) (i:seq_index il)
+  : Lemma (ensures  (
+    let il_i = prefix il (i + 1) in
     let tid, j = i2s_map il i in
-    let il_i_tid = Seq.index (s_seq il_i) tid in
-    i2s_prefix_length il i
+    Seq.index (s_seq il_i) tid `Seq.equal`
+    SA.prefix (Seq.index (s_seq il) tid) (j + 1)))
+    (decreases IL?.prf il)
+  = let IL is ss prf = il in
+    match prf with
+    | IntEmpty -> false_elim()
+    | IntAdd _ ss' prf' -> interleave_sseq_index_next (IL _ ss' prf') i
+    | IntExtend is' ss' prf' x j ->
+      if i = Seq.length is'
+      then ()
+      else (
+        interleave_sseq_index_next (IL _ _ prf') i
+      )
+
 
